LiftSigma mit mehreren defaults

TM/LiftSigmaTau.v
@@ -9,46 +9,34 @@ Section SujectTape.
   Definition surject : tau -> sig := fun t => match (g t) with Some s => s | None => def end.
 
   Definition surjectTape := mapTape surject.
-  Definition surjectTapes {n : nat} := mapTapes (n := n) surject.
-
-  (*
-  Lemma surjectTapes_nth {n : nat} (k : Fin.t n) (ts : tapes tau n) :
-    (surjectTapes ts)[@k] = surjectTape(ts[@k]).
-  Proof. unfold surjectTapes. now simpl_tape. Qed.
-   *)
 
 End SujectTape.
 
-Arguments surjectTapes : simpl never.
-(*
-Hint Rewrite surjectTapes_nth : tape.
-*)
-Hint Unfold surjectTape surjectTapes : tape.
+Hint Unfold surjectTape : tape.
 
 Section lift_sigma_tau.
   Variable n : nat.
   Variable sig tau : finType.
   Variable g : tau -> option sig.
-  Variable def : sig.
-  Variable Z : Type.
-  
-  Definition lift_sigma_tau (R : Rel (Vector.t (tape sig) n) (Vector.t (tape sig) n)) :
-    Rel (Vector.t (tape tau) n) (Vector.t (tape tau) n) :=
-    fun x y => R (surjectTapes g def x) (surjectTapes g def y).
+  Variable def : Vector.t sig n.
+  Variable F : Type.
 
-  Definition lift_sigma_tau_p (R : Rel (Vector.t (tape sig) n) (Z * Vector.t (tape sig) n)) :
-    Rel (Vector.t (tape tau) n) (Z * Vector.t (tape tau) n) :=
-    fun x '(z,y) => R (surjectTapes g def x) (z, surjectTapes g def y).
+  Definition surjectTapes : tapes tau n -> tapes sig n :=
+     Vector.map2 (fun d t => surjectTape g d t) def.
+  
+  Definition lift_sigma_tau_Rel (R : Rel (tapes sig n) (F * tapes sig n)) :
+    Rel (tapes tau n) (F * tapes tau n) :=
+    fun tin '(yout,tout) => R (surjectTapes tin) (yout, surjectTapes tout).
 
   Definition lift_sigma_tau_T (T : Rel (Vector.t (tape sig) n) nat) :
     Rel (Vector.t (tape tau) n) nat :=
-    fun x k => T (surjectTapes g def x) k.
+    fun tin k => T (surjectTapes tin) k.
 
 End lift_sigma_tau.
 
-Arguments lift_sigma_tau { n sig tau } ( g def R ) x y /.
-Arguments lift_sigma_tau_p { n sig tau } ( g def ) { Z } ( R ) x y /.
-Arguments lift_sigma_tau_T { n sig tau } ( g def T ) x y /.
+
+Arguments lift_sigma_tau_Rel {n sig tau} (g def) {F} (R) x y /.
+Arguments lift_sigma_tau_T {n sig tau} (g def T) x y /.
 
 
 Section InjectTape.
@@ -84,6 +72,7 @@ Section InjectSurject.
     destruct t; cbn; f_equal; try rewrite retract_g_adjoint; auto; apply surject_inject'.
   Qed.
 
+  (*
   Lemma surject_inject_tapes {n : nat} (t : Vector.t (tape sig) n) :
     surjectTapes g def (injectTapes f t) = t.
   Proof.
@@ -92,6 +81,7 @@ Section InjectSurject.
     erewrite !Vector.nth_map; eauto.
     apply surject_inject_tape.
   Qed.
+*)
   
 End InjectSurject.
 
@@ -107,78 +97,77 @@ Section LiftSigmaTau.
   Variable F : finType.
   Variable pMSig : { M : mTM sig n & states M -> F}.
 
-  Variable (f : sig -> tau) (g : tau -> option sig).
-  Hypothesis I : retract f g.
-  Variable def : sig.
-  Definition g' : tau -> sig := surject g def.
+  Variable Inj : Retract sig  tau.
 
+  Variable def : Vector.t sig n.
+
+  Definition surjectReadSymbols : Vector.t (option tau) n -> Vector.t (option sig) n :=
+    fun sym =>
+      Vector.map2 (fun d => map_opt (surject Retr_g d)) def sym.
 
   Definition lift_trans :=
-    fun '(q, symm) =>
-      let (q', act) := trans (m := projT1 pMSig) (q, Vector.map (map_opt g') symm) in
-      (q', Vector.map (map_act f) act).
+    fun '(q, sym) =>
+      let (q', act) := trans (m := projT1 pMSig) (q, surjectReadSymbols sym) in
+      (q', Vector.map (map_act Retr_f) act).
 
-  Definition liftM : mTM tau n.
-  Proof.
-    econstructor.
-    exact lift_trans.
-    exact (start (projT1 pMSig)).
-    exact (halt (m := projT1 pMSig)).
-  Defined.
+  Definition liftM : mTM tau n :=
+    {| trans := lift_trans;
+       start := start (projT1 pMSig);
+       halt := halt (m := projT1 pMSig) |}.
 
   Definition Lift := (liftM; projT2 pMSig).
+
+
+  (* End definition *)
 
   Ltac dup H := let H' := fresh H in pose proof H as H'.
 
   Lemma surject_step :
-    forall (tape : tape tau) (act : option sig * move),
-      tape_move_mono (mapTape (surject g def) tape) act =
-      mapTape (surject g def)
-              (tape_move_mono tape (map_act f act)).
+    forall (tape : tape tau) (act : option sig * move) (d : sig),
+      tape_move_mono (surjectTape Retr_g d tape) act =
+      surjectTape Retr_g d (tape_move_mono tape (map_act Retr_f act)).
   Proof.
-    intros tape. intros (w,m).
-    unfold tape_move_mono, tape_move, tape_write, surject. cbn.
-    destruct tape; cbn;
-      try (destruct m, w; cbn; f_equal; now rewrite retract_g_adjoint).
-    destruct m, w; cbn.
-    - unfold mapTape. cbn. destruct l; cbn; f_equal; now rewrite retract_g_adjoint.
-    - unfold mapTape. cbn. destruct l; cbn; f_equal; now rewrite retract_g_adjoint.
-    - unfold mapTape. cbn. destruct l, l0; cbn; f_equal; now rewrite retract_g_adjoint.
-    - unfold mapTape. cbn. destruct l, l0; cbn; f_equal; now rewrite retract_g_adjoint.
-    - unfold mapTape. cbn. destruct l, l0; cbn; f_equal; now rewrite retract_g_adjoint.
-    - unfold mapTape. cbn. destruct l, l0; cbn; f_equal; now rewrite retract_g_adjoint.
+    intros tape. intros (w,m) d; cbn.
+    unfold surjectTape, tape_move_mono, tape_move, tape_write, surject; cbn.
+    destruct tape, m, w; cbn; f_equal; try retract_adjoint; auto.
+    - destruct l; cbn; f_equal; now retract_adjoint.
+    - destruct l; cbn; f_equal; now retract_adjoint.
+    - destruct l0; cbn; f_equal; now retract_adjoint.
+    - destruct l0; cbn; f_equal; now retract_adjoint.
   Qed.
+
 
   Lemma sim_step (c1 c2 : mconfig tau (states (projT1 pMSig)) n) :
     step (M := liftM) c1 = c2 ->
-    step (M := projT1 pMSig) (mk_mconfig (cstate c1) (surjectTapes g def (ctapes c1))) =
-    (mk_mconfig (cstate c2) (surjectTapes g def (ctapes c2))).
+    step (M := projT1 pMSig) (mk_mconfig (cstate c1) (surjectTapes Retr_g def (ctapes c1))) =
+    (mk_mconfig (cstate c2) (surjectTapes Retr_g def (ctapes c2))).
   Proof.
     intros H. cbn.
     destruct c1 as [state1 tapes1] eqn:E1, c2 as [state2 tapes2] eqn:E2.
     cbv [step] in *. cbn -[map step] in *.
-    destruct (trans (state1, Vector.map (map_opt g') (current_chars tapes1))) as (q, act) eqn:E3.
+    destruct (trans (state1, surjectReadSymbols (current_chars tapes1))) as (q, act) eqn:E3.
     inv H.
-    destruct (trans (state1, current_chars (surjectTapes g def tapes1)))
-      as (q', act') eqn:E4.
+    destruct (trans (state1, current_chars _)) as (q', act') eqn:E4.
     enough ((state2, act) = (q', act')) as X.
     {
       inv X. f_equal.
       unfold surjectTapes, mapTapes. apply Vector.eq_nth_iff. intros p ? <-.
-      erewrite !Vector.nth_map, !Vector.nth_map2, !Vector.nth_map; eauto.
+      erewrite !Vector.nth_map2, !Vector.nth_map; eauto.
       apply surject_step.
     }
     rewrite <- E3, <- E4. do 2 f_equal.
-    apply Vector.eq_nth_iff. intros p ? <-.
-    unfold surjectTapes, mapTapes, surject, current.
-    autounfold with tape. erewrite !Vector.nth_map; eauto. cbn.
-    destruct (tapes1[@p]) eqn:E5; cbn; auto.
+
+    unfold surjectReadSymbols, current_chars.
+    apply Vector.eq_nth_iff; intros p ? <-.
+    unfold surjectTapes, mapTapes, surject. autounfold with tape.
+    erewrite !Vector.nth_map2, !Vector.nth_map; eauto. cbn.
+    simpl_tape. destruct (tapes1[@p]) eqn:E5; cbn; auto.
   Qed.
 
   Lemma sim_loop (c1 c2 : mconfig tau (states liftM) n) (i : nat) :
     loopM (M := liftM) i c1 = Some c2 ->
-    loopM (M := projT1 pMSig) i (mk_mconfig (cstate c1) (surjectTapes g def (ctapes c1))) =
-    Some (mk_mconfig (cstate c2) (surjectTapes g def (ctapes c2))).
+    loopM (M := projT1 pMSig) i (mk_mconfig (cstate c1) (surjectTapes Retr_g def (ctapes c1))) =
+    Some (mk_mconfig (cstate c2) (surjectTapes Retr_g def (ctapes c2))).
   Proof.
     unfold loopM in *. revert c2 c1. induction i; intros c2 c1 H; cbn in *.
     - destruct (halt _) eqn:E; now inv H.
@@ -189,45 +178,42 @@ Section LiftSigmaTau.
 
   Lemma Lift_WRealise (R : Rel (tapes sig n) (F * tapes sig n)) :
     pMSig ⊫ R ->
-    Lift ⊫ lift_sigma_tau_p g def R.
+    Lift ⊫ lift_sigma_tau_Rel Retr_g def R.
   Proof.
-    intros H. intros t i outc Hloop. unfold lift_sigma_tau_p.
-    apply (H (surjectTapes g def t) i (mk_mconfig (cstate outc) (surjectTapes g def (ctapes outc)))).
+    intros H. intros t i outc Hloop. unfold lift_sigma_tau_Rel. hnf in H.
+    specialize (H (surjectTapes Retr_g def t) i (mk_mconfig (cstate outc) (surjectTapes Retr_g def (ctapes outc)))).
+    cbn in H. apply H.
     now apply (@sim_loop (initc liftM t) outc i).
   Qed.
 
   Definition surjectConf : (mconfig tau (states liftM) n) -> (mconfig sig (states (projT1 pMSig)) n) :=
-    fun c => mk_mconfig (cstate c) (surjectTapes g def (ctapes c)).
+    fun c => mk_mconfig (cstate c) (surjectTapes Retr_g def (ctapes c)).
 
   Definition injectConf : (mconfig sig (states (projT1 pMSig)) n) -> (mconfig tau (states liftM) n) :=
-    fun c => mk_mconfig (cstate c) (injectTapes f (ctapes c)).
+    fun c => mk_mconfig (cstate c) (injectTapes Retr_f (ctapes c)).
+
+
 
   Lemma propagate_step (conf : (mconfig tau (states (projT1 pMSig)) n)) :
     surjectConf (step (M := liftM) conf) = step (surjectConf conf).
   Proof.
     cbv [surjectConf]. cbv [step]. cbn.
-    replace (Vector.map (map_opt g') (current_chars (ctapes conf))) with (current_chars (surjectTapes g def (ctapes conf))).
-    - cbn. destruct (trans (cstate conf, current_chars (surjectTapes g def (ctapes conf)))) eqn:E1; cbn.
+    replace (surjectReadSymbols (current_chars (ctapes conf))) with
+        (current_chars (surjectTapes Retr_g def (ctapes conf))).
+    - destruct (trans (cstate conf, current_chars (surjectTapes Retr_g def (ctapes conf)))) eqn:E1; cbn.
       f_equal. unfold surjectTapes, mapTapes. apply Vector.eq_nth_iff. intros ? ? <-.
-      unfold tape_move_multi, tape_move_mono.
+      unfold tape_move_multi.
       repeat first [erewrite !Vector.nth_map2; eauto | erewrite !Vector.nth_map; eauto].
       cbv [surject]. cbn.
       destruct (t[@p1]) eqn:E2; cbn. generalize ((ctapes conf)[@p1]) as t1. intros t1. cbn.
-      destruct o; cbn.
-      + destruct m; cbn; simpl_tape. destruct (left t1) eqn:E3; cbn.
-        * retract_adjoint. auto.
-        * f_equal. retract_adjoint. auto.
-        * destruct (right t1) eqn:E3; cbn.
-          -- retract_adjoint. cbn. auto.
-          -- retract_adjoint. auto.
-        * f_equal. now retract_adjoint.
-      + destruct m; cbn; simpl_tape; auto.
-    - eapply Vector.eq_nth_iff. intros ? ? <-. unfold current_chars, surjectTapes, mapTapes.
+      symmetry. apply surject_step.
+    - eapply Vector.eq_nth_iff. intros ? ? <-.
+      unfold current_chars, surjectTapes, mapTapes, surjectReadSymbols, surjectTape.
       erewrite !Vector.nth_map; simpl_tape; eauto. reflexivity.
   Qed.
 
   Lemma propagate_loop (k : nat) tin (conf : mconfig sig (states (projT1 pMSig)) n) :
-    loopM k (initc (projT1 pMSig) (surjectTapes g def tin)) = Some conf ->
+    loopM k (initc (projT1 pMSig) (surjectTapes Retr_g def tin)) = Some conf ->
     exists oconf' : (mconfig tau (states liftM) n),
       loopM k (initc liftM tin) = Some oconf'.
   Proof.
@@ -248,7 +234,7 @@ Section LiftSigmaTau.
 
   Lemma Lift_TerminatesIn (T : Rel (tapes sig n) nat) :
     projT1 pMSig ↓ T ->
-    liftM ↓ lift_sigma_tau_T g def T.
+    liftM ↓ lift_sigma_tau_T Retr_g def T.
   Proof.
     intros H. hnf. intros tin k HTerm. hnf in HTerm, H. specialize (H _ _ HTerm) as (oconf&HLoop).
     eapply propagate_loop; eauto.
@@ -256,7 +242,7 @@ Section LiftSigmaTau.
 
   Lemma Lift_RealiseIn (R : Rel (tapes sig n) (F * tapes sig n)) (k : nat) :
     pMSig ⊨c(k) R ->
-    Lift ⊨c(k) lift_sigma_tau_p g def R.
+    Lift ⊨c(k) lift_sigma_tau_Rel Retr_g def R.
   Proof.
     intros [H1 H2] % Realise_total. eapply Realise_total. split; cbn in *.
     - now eapply Lift_WRealise.
